Generate match patterns from IRExpr

Semantics/TermRewrites.thy
@@ -12,25 +12,56 @@ proof -
 qed
 *)
 
-lemma expr_at_node: "g \<turnstile> n \<simeq> (g @@ n)"
-  using expr_at_node.simps repDet sorry
+fun expr_at_node :: "IRGraph \<Rightarrow> ID \<Rightarrow> IRExpr"
+  (infix "@@" 50) where
+  "expr_at_node g n = (SOME e . (g \<turnstile> n \<simeq> e))"
+                          
+lemma expr_at_node: "g \<turnstile> n \<simeq> e \<Longrightarrow> g \<turnstile> n \<simeq> (g @@ n)"
+  using expr_at_node.simps repDet 
+  by (simp add: someI)
 
 lemma graph_refinement:
   "graph_refinement g1 g2 \<Longrightarrow> (\<forall>n m p v. n \<in> ids g1 \<longrightarrow> ([g1, m, p] \<turnstile> n \<mapsto> v) \<longrightarrow> ([g2, m, p] \<turnstile> n \<mapsto> v))"
   unfolding graph_refinement_def expr_at_node.simps
-  apply auto
+  apply auto[1]
   using expr_at_node.simps encodeeval_def graph_refinement_def le_expr_def 
-  by (metis expr_at_node repDet)
+  by (meson term_graph_evaluation)
 
-datatype SubValue = SubExpr(s_expr: IRExpr) | SubConst(s_val: Value) | SubNone
+datatype SubValue = SubExpr(s_expr: IRExpr) | SubConst(s_val: Value)
 
-type_synonym Substitution = "string \<Rightarrow> SubValue"
+typedef Substitution = "{s :: String.literal \<rightharpoonup> SubValue . finite (dom s)}"
+  using finite_dom_map_of by blast
 
-fun dom :: "Substitution \<Rightarrow> string set" where
-  "dom \<sigma> = { s . \<sigma> s \<noteq> SubNone }"
+setup_lifting type_definition_Substitution
 
-lemma in_dom: "x \<in> dom \<sigma> \<Longrightarrow> \<sigma> x \<noteq> SubNone"
-  by simp
+lift_definition subst :: "(String.literal \<times> SubValue) list \<Rightarrow> Substitution"
+  is "map_of"
+  by (simp add: finite_dom_map_of)
+
+lift_definition subst_set :: "Substitution \<Rightarrow> (String.literal \<times> SubValue) set"
+  is "Map.graph" .
+
+lemma subst_reconstruct:
+  "distinct (map fst x) \<Longrightarrow> set x = subst_set (subst x)"
+  by (simp add: graph_map_of_if_distinct_dom subst.rep_eq subst_set.rep_eq)
+
+lift_definition dom :: "Substitution \<Rightarrow> String.literal set"
+  is Map.dom .
+
+lift_definition maps_to :: "Substitution \<Rightarrow> String.literal \<Rightarrow> SubValue option"
+  is "\<lambda> \<sigma> x . \<sigma> x" .
+
+code_datatype subst Abs_Substitution
+
+lemma [code]: "Rep_Substitution (subst m) = map_of m"
+  using Abs_Substitution_inverse
+  using subst.rep_eq by blast
+
+lemma dom_code[code]: "dom (subst m) = set (map fst m)"
+  by (simp add: dom.rep_eq dom_map_of_conv_image_fst subst.rep_eq)
+
+lemma in_dom: "x \<in> dom \<sigma> \<Longrightarrow> maps_to \<sigma> x \<noteq> None"
+  by (simp add: dom.rep_eq domIff maps_to.rep_eq)
   
 fun substitute :: "Substitution \<Rightarrow> IRExpr \<Rightarrow> IRExpr" (infix "$" 60) where
   "substitute \<sigma> (UnaryExpr op e) = UnaryExpr op (\<sigma> $ e)" |
@@ -40,15 +71,106 @@ fun substitute :: "Substitution \<Rightarrow> IRExpr \<Rightarrow> IRExpr" (infi
   "substitute \<sigma> (LeafExpr n s) = LeafExpr n s" |
   "substitute \<sigma> (ConstantExpr v) = ConstantExpr v" |
   "substitute \<sigma> (ConstantVar x) = 
-      (case \<sigma> x of SubConst v \<Rightarrow> ConstantExpr v | _ \<Rightarrow> ConstantVar x)" |
+      (case maps_to \<sigma> x of Some (SubConst v) \<Rightarrow> ConstantExpr v | _ \<Rightarrow> ConstantVar x)" |
   "substitute \<sigma> (VariableExpr x s) = 
-      (case \<sigma> x of SubNone \<Rightarrow> (VariableExpr x s) | SubExpr y \<Rightarrow> y)"
+      (case maps_to \<sigma> x of None \<Rightarrow> (VariableExpr x s) | Some (SubExpr y) \<Rightarrow> y)"
 
-fun union :: "Substitution \<Rightarrow> Substitution \<Rightarrow> Substitution" where
-  "union \<sigma>1 \<sigma>2 = (\<lambda>name. if \<sigma>1 name = SubNone then \<sigma>2 name else \<sigma>1 name)"
+lift_definition union :: "Substitution \<Rightarrow> Substitution \<Rightarrow> Substitution"
+  is "\<lambda>\<sigma>1 \<sigma>2. \<sigma>1 ++ \<sigma>2"
+  by simp
+
+(*fun union :: "Substitution \<Rightarrow> Substitution \<Rightarrow> Substitution" where
+  "union \<sigma>1 \<sigma>2 = Abs_Substitution (\<lambda>name. if maps_to \<sigma>1 name = None then maps_to \<sigma>2 name else maps_to \<sigma>1 name)"
+*)
+
+lemma not_empty_has_member:
+  assumes "xs \<noteq> []"
+  shows "\<exists> k v. List.member xs (k, v)"
+  using assms apply (cases xs; auto)
+  by (meson member_rec(1))
+
+value "map_of ([(x, xv1), (y, yv)] @ [(z, zv), (x, xv2)]) x"
+
+lemma equal_mapping_implies_equal:
+  assumes "\<forall>k. maps_to \<sigma>1 k = maps_to \<sigma>2 k"
+  shows "\<sigma>1 = \<sigma>2"
+  using assms unfolding maps_to_def using Rep_Substitution
+  by (metis Rep_Substitution_inverse ext id_def map_fun_apply)
+
+(*
+lemma 
+  "maps_to (union (subst \<sigma>1) (subst \<sigma>2)) k = maps_to (subst (\<sigma>1 @ \<sigma>2)) k"
+  (is "maps_to ?union k = maps_to ?add k")
+proof (cases "\<exists> v. List.member \<sigma>1 (k, v)"; cases "\<exists> v. List.member \<sigma>2 (k, v)")
+  case True \<comment>\<open>key has mapping in both\<close>
+  then show ?thesis sorry
+next
+  case False \<comment>\<open>key in \<sigma>1 but not \<sigma>2\<close>
+  then show ?thesis sorry
+next
+  \<comment>\<open>key in \<sigma>2 but not \<sigma>1\<close>
+  assume a1: "\<nexists>v. List.member \<sigma>1 (k, v)"
+  assume a2: "\<exists>v. List.member \<sigma>2 (k, v)"
+  obtain v where v: "List.member \<sigma>2 (k, v)"
+    using a2 by auto
+  from a1 v have "maps_to ?add k = Some v"
+    unfolding maps_to_def subst_def using map_of_append sledgehammer
+  then show ?thesis sorry
+next
+  \<comment>\<open>key in neither\<close>
+  assume a1: "\<nexists>v. List.member \<sigma>1 (k, v)"
+  assume a2: "\<nexists>v. List.member \<sigma>2 (k, v)"
+  from a1 a2 have "maps_to ?add k = None"
+    by (metis domD in_set_member map_add_dom_app_simps(2) map_of_SomeD map_of_append maps_to.rep_eq opt_to_list.cases option.discI subst.rep_eq)
+  then show ?thesis
+    by (metis map_add_None map_of_append maps_to.rep_eq subst.rep_eq union.rep_eq)
+qed
+*)
+
+lemma union_code[code]:
+  "union (subst \<sigma>1) (subst \<sigma>2) = (subst (\<sigma>2 @ \<sigma>1))"
+  (is "?union = ?add")
+  using map_of_append unfolding subst_def union_def
+  using subst.abs_eq subst.rep_eq by auto
+
+(*
+proof (cases "\<sigma>1 = []")
+  case True
+  then show ?thesis
+    by (metis Rep_Substitution_inverse append.right_neutral append_Nil map_of_append subst.rep_eq union.rep_eq)
+next
+  case False
+  then obtain k v where v: "List.member \<sigma>1 (k, v)"
+    using not_empty_has_member by blast
+  show ?thesis
+  proof (cases "\<exists>v. List.member \<sigma>2 (k, v)")
+    case True
+    obtain v' where v': "List.member \<sigma>2 (k, v')"
+      using True
+      by blast
+    have rhs: "maps_to (?add) k = Some v"
+      using v v' unfolding maps_to_def subst_def sorry
+    have lhs: "maps_to (?union) k = Some v"
+      sorry
+    from lhs rhs have "maps_to (?add) k = maps_to (?union) k"
+      sorry
+    then show ?thesis using equal_mapping_implies_equal sorry
+  next
+    case False
+    then show ?thesis
+      by simp
+  qed
+qed
+  
+  apply (induction \<sigma>1; induction \<sigma>2; auto)
+  apply (metis append_Nil map_of_append subst.abs_eq subst.rep_eq)
+  apply (metis map_of_append self_append_conv subst.abs_eq subst.rep_eq)
+   apply (metis append_Nil map_of_append subst.abs_eq subst.rep_eq)
+  sorry
+*)
 
 fun compatible :: "Substitution \<Rightarrow> Substitution \<Rightarrow> bool" where
-  "compatible \<sigma>1 \<sigma>2 = (\<forall>x. \<sigma>1 x \<noteq> SubNone \<and> \<sigma>2 x \<noteq> SubNone \<longrightarrow> \<sigma>1 x = \<sigma>2 x)"
+  "compatible \<sigma>1 \<sigma>2 = (\<forall>x \<in> dom \<sigma>1. maps_to \<sigma>2 x \<noteq> None \<longrightarrow> maps_to \<sigma>1 x = maps_to \<sigma>2 x)"
 
 fun substitution_union :: "Substitution option \<Rightarrow> Substitution option \<Rightarrow> Substitution option" (infix "\<uplus>" 70) where
   "substitution_union s1 s2 = 
@@ -61,8 +183,10 @@ fun substitution_union :: "Substitution option \<Rightarrow> Substitution option
            )
       )"
 
+(*lemma "sup x y = x"*)
+
 definition EmptySubstitution :: "Substitution" where 
-  "EmptySubstitution = (\<lambda>x. SubNone)"
+  "EmptySubstitution = subst []"
 
 fun match :: "IRExpr \<Rightarrow> IRExpr \<Rightarrow> Substitution option" where
   "match (UnaryExpr op e) (UnaryExpr op' e') = 
@@ -78,130 +202,461 @@ fun match :: "IRExpr \<Rightarrow> IRExpr \<Rightarrow> Substitution option" whe
   "match (ConstantExpr v1) (ConstantExpr v2) = 
       (if v1 = v2 then Some EmptySubstitution else None)" |
   "match (ConstantVar name) (ConstantExpr v) = 
-      Some(\<lambda>x. if x = name then SubConst v else SubNone)" |
-  "match (VariableExpr x s) e = Some (\<lambda> n. if n = x then SubExpr e else SubNone)" |
+      Some (subst [(name, (SubConst v))])" |
+  "match (VariableExpr name s) e = 
+      Some (subst [(name, (SubExpr e))])" |
   "match _ _ = None"
 
 
-fun vars :: "IRExpr \<Rightarrow> string set" where
+fun vars :: "IRExpr \<Rightarrow> String.literal fset" where
   "vars (UnaryExpr op e) = vars e" |
-  "vars (BinaryExpr op e1 e2) = vars e1 \<union> vars e2" |
-  "vars (ConditionalExpr b e1 e2) = vars b \<union> vars e1 \<union> vars e2" |
-  "vars (ParameterExpr i s) = {}" |
-  "vars (LeafExpr n s) = {}" |
-  "vars (ConstantExpr v) = {}" |
-  "vars (ConstantVar x) = {x}" |
-  "vars (VariableExpr x s) = {x}"
+  "vars (BinaryExpr op e1 e2) = vars e1 |\<union>| vars e2" |
+  "vars (ConditionalExpr b e1 e2) = vars b |\<union>| vars e1 |\<union>| vars e2" |
+  "vars (ParameterExpr i s) = {||}" |
+  "vars (LeafExpr n s) = {||}" |
+  "vars (ConstantExpr v) = {||}" |
+  "vars (ConstantVar x) = {|x|}" |
+  "vars (VariableExpr x s) = {|x|}"
 
-typedef Rewrite = "{ (e1,e2) :: IRExpr \<times> IRExpr | e1 e2 . vars e2 \<subseteq> vars e1 }" 
+typedef Rewrite = "{ (e1,e2,cond) :: IRExpr \<times> IRExpr \<times> (Substitution \<Rightarrow> bool) | e1 e2 cond . vars e2 |\<subseteq>| vars e1 }" 
 proof -
-  have "\<exists>v. vars (ConstantExpr v) \<subseteq> vars (ConstantExpr v)" by simp
+  have "\<exists>v. vars (ConstantExpr v) |\<subseteq>| vars (ConstantExpr v)" by simp
   then show ?thesis
     by blast
 qed
 
+setup_lifting type_definition_Rewrite
+
+
+fun construct_rewrite :: "IRExpr \<times> IRExpr \<times> (Substitution \<Rightarrow> bool) \<Rightarrow> Rewrite option" where
+  "construct_rewrite (e1, e2, cond) =
+    (if vars e2 |\<subseteq>| vars e1 then Some (Abs_Rewrite (e1, e2, cond)) else None)"
+
+code_datatype Abs_Rewrite
+
+lemma "Abs_Rewrite (Rep_Rewrite r) = r"
+  by (simp add: Rep_Rewrite_inverse)
+
+lemma [code]: "Rep_Rewrite (Abs_Rewrite (e1, e2)) = (e1, e2)"
+  sorry
+
 fun rewrite :: "Rewrite \<Rightarrow> IRExpr \<Rightarrow> IRExpr option" where
-  "rewrite r e = (let (e1,e2) = Rep_Rewrite r in 
+  "rewrite r e = (let (e1,e2,cond) = Rep_Rewrite r in 
                    (case match e1 e of
-                    Some \<sigma> \<Rightarrow> Some (\<sigma> $ e2) |
+                    Some \<sigma> \<Rightarrow> 
+                      (if cond \<sigma> then Some (\<sigma> $ e2) else None) |
                     None \<Rightarrow> None))"
 
 definition rewrite_valid :: "Rewrite \<Rightarrow> bool" where
-  "rewrite_valid r = (let (e1,e2) = Rep_Rewrite r in
+  "rewrite_valid r = (let (e1,e2,cond) = Rep_Rewrite r in
     (\<forall>\<sigma> e. is_ground e \<longrightarrow> match e1 e = Some \<sigma> \<longrightarrow> (e \<ge> (\<sigma> $ e2))))"
 
 definition rewrite_valid_rep :: "IRExpr \<Rightarrow> IRExpr \<Rightarrow> bool" where
-  "rewrite_valid_rep e1 e2 = (vars e1 \<subseteq> vars e2 \<longrightarrow> (\<forall>\<sigma> e.  match e1 e = Some \<sigma> \<longrightarrow> (e \<ge> (\<sigma> $ e2))))"
+  "rewrite_valid_rep e1 e2 = (vars e1 |\<subseteq>| vars e2 \<longrightarrow> (\<forall>\<sigma> e.  match e1 e = Some \<sigma> \<longrightarrow> (e \<ge> (\<sigma> $ e2))))"
 
 definition IntStamp32 :: Stamp where 
   "IntStamp32 = IntegerStamp 32 (fst (bit_bounds 32)) (snd (bit_bounds 32))"
 
+fun pattern_depth :: "IRExpr \<Rightarrow> nat" where
+  "pattern_depth (UnaryExpr op e) = 1 + pattern_depth e" |
+  "pattern_depth (BinaryExpr op e1 e2) = 1 + max (pattern_depth e1) (pattern_depth e2)" |
+  "pattern_depth (ConditionalExpr b e1 e2) = 1 + max (pattern_depth b) (max (pattern_depth e1) (pattern_depth e2))" |
+  "pattern_depth (ParameterExpr i s) = 1" |
+  "pattern_depth (LeafExpr n s) = 1" |
+  "pattern_depth (ConstantExpr v) = 1" |
+  "pattern_depth (ConstantVar x) = 0" |
+  "pattern_depth (VariableExpr x s) = 0"
+
+value "pattern_depth (ConstantExpr (IntVal 32 0))"
+value "pattern_depth (VariableExpr (STR ''x'') VoidStamp)"
+value "pattern_depth (UnaryExpr UnaryAbs (ConstantExpr (IntVal 32 0)))"
+value "pattern_depth (UnaryExpr UnaryAbs (VariableExpr (STR ''x'') VoidStamp))"
+value "pattern_depth (UnaryExpr UnaryAbs (UnaryExpr UnaryNot (VariableExpr (STR ''x'') VoidStamp)))"
+value "pattern_depth (BinaryExpr BinAdd (UnaryExpr UnaryNot (VariableExpr (STR ''x'') VoidStamp)) (VariableExpr (STR ''x'') VoidStamp))"
+value "pattern_depth (BinaryExpr BinAdd (UnaryExpr UnaryNot (ConstantExpr (IntVal 32 0))) (VariableExpr (STR ''x'') VoidStamp))"
+value "pattern_depth (BinaryExpr BinAdd (VariableExpr (STR ''x'') VoidStamp) (VariableExpr (STR ''x'') VoidStamp))"
+
+(*fun fresh :: "String.literal \<Rightarrow> IRExpr \<Rightarrow> String.literal" where
+  "fresh var e = var"*)
+
+type_synonym VarName = "String.literal"
+
+datatype PatternExpr =
+    UnaryPattern IRUnaryOp VarName
+  | BinaryPattern IRBinaryOp VarName VarName
+  | ConditionalPattern VarName VarName VarName
+  | VariablePattern VarName
+
+type_synonym Vars = "VarName fset"
+
+(*
+function fresh :: "VarName \<Rightarrow> Vars \<Rightarrow> VarName" where
+  "fresh var s = (if var |\<in>| s then fresh (var + (STR ''z'')) s else var)"
+   apply force
+  by fastforce
+
+lemma fresh_var_code [code]:
+  "fresh var s = (if var |\<in>| s then fresh (var + (STR ''z'')) s else (var))"
+  sorry
+*)
+
+type_synonym Scope = "Vars \<times> (VarName \<Rightarrow> VarName option)"
+
+function fresh :: "VarName \<Rightarrow> Scope \<Rightarrow> Scope \<times> VarName" where
+  "fresh var s = 
+    (if var |\<in>| (fst s) then fresh (var + (STR ''z'')) s else (((fst s) |\<union>| {|var|}, snd s), var))"
+   apply force
+  by fastforce
+
+lemma fresh_var_code [code]:
+  "fresh var s = (if var |\<in>| (fst s) then fresh (var + (STR ''z'')) s else (((fst s) |\<union>| {|var|}, snd s), var))"
+  sorry
+
+(*
+typedef PatternExpr = "{ e :: IRExpr . pattern_depth e \<le> 1 }"
+  by (metis mem_Collect_eq pattern_depth.simps(8) zero_le)
+
+code_datatype Abs_PatternExpr
+*)
+
+datatype MATCH =
+    match VarName PatternExpr |
+    equality VarName VarName ("_ == _") |
+    seq MATCH MATCH ("_; _") |
+    noop
+
+datatype CODE =
+    code MATCH IRExpr ("_ ? _")
+
+type_synonym VariablePairs = "(VarName \<times> VarName) list"
+
+type_synonym Symbols = "VariablePairs \<times> Vars"
+
+value
+  "(match (STR ''e'') (BinaryPattern BinAdd (STR ''ea'') (STR ''eb''));
+   (match (STR ''ea'') (BinaryPattern BinSub (STR ''eaa'') (STR ''eab''));
+   ((STR ''eab'') == (STR ''eb'')))) ? (VariableExpr (STR ''ea'') default_stamp)"
+
+definition var :: "string \<Rightarrow> IRExpr" where
+  "var v = (VariableExpr (String.implode v) VoidStamp)"
+
+(*
+definition la :: "(VarName \<Rightarrow> 'a) \<Rightarrow> (Vars \<Rightarrow> VarName \<times> Vars) \<Rightarrow> (Vars \<Rightarrow> 'a \<times> Vars)" (infix "\<langle>" 65)
+  where
+  "la f f' s = (f (fst (f' s)), snd (f' s))"
+
+definition ra :: "(Vars \<Rightarrow> ('b \<Rightarrow> 'a) \<times> Vars) \<Rightarrow> (Vars \<Rightarrow> ('b \<times> Vars)) \<Rightarrow> (Vars \<Rightarrow> 'a \<times> Vars)" (infix "\<rangle>" 60)
+  where
+  "ra f f' s = ((fst (f s)) (fst (f' s)), snd (f s))"
+
+fun test :: "IRExpr \<Rightarrow> Vars \<Rightarrow> MATCH \<times> Vars" where
+  "test (UnaryExpr op e) =
+    match \<langle> fresh STR ''e'' \<rangle>
+      UnaryPattern op \<langle> fresh STR ''ea''" |
+  "test (BinaryExpr op e1 e2) =
+    match \<langle> fresh STR ''e'' \<rangle>
+      (BinaryPattern op \<langle> fresh STR ''ea'' \<rangle> (fresh STR ''eb''))" |
+  "test (ConditionalExpr b e1 e2) =
+    match \<langle> fresh STR ''e'' \<rangle>
+      ((ConditionalPattern \<langle> fresh STR ''ea'' \<rangle> (fresh STR ''eb'')) \<rangle> (fresh STR ''ec''))"
+*)
+
+definition la :: "('b \<Rightarrow> 'a) \<Rightarrow> (Scope \<Rightarrow> Scope \<times> 'b) \<Rightarrow> (Scope \<Rightarrow> Scope \<times> 'a)" (infix "\<langle>" 65)
+  where
+  "la f f' s = (fst (f' s), f (snd (f' s)))"
+
+(*
+definition ra :: "('b \<Rightarrow> 'a) \<Rightarrow> (Scope \<Rightarrow> Scope \<times> 'b) \<Rightarrow> (Scope \<Rightarrow> Scope \<times> 'a)" (infix "\<rangle>" 54)
+  where
+  "ra f f' s = ((fst (f' (s))), f (snd (f' s)))"
+*)
+
+definition ra :: "(Scope \<Rightarrow> Scope \<times> ('b \<Rightarrow> 'a)) \<Rightarrow> (Scope \<Rightarrow> Scope \<times> 'b) \<Rightarrow> (Scope \<Rightarrow> Scope \<times> 'a)" (infix "\<rangle>" 54)
+  where
+  "ra f f' s = ((fst (f' (fst (f s)))), (snd (f s)) (snd (f' (fst (f s)))))"
+
+definition join :: "('b \<Rightarrow> 'c \<times> MATCH) \<Rightarrow> ('b \<Rightarrow> 'c \<Rightarrow> 'a \<times> MATCH) \<Rightarrow> 'b \<Rightarrow> 'a \<times> MATCH" (infix "|>" 53) where
+  "join x y s = 
+    (let (lhs_scope, lhs_match) = x s in
+    (let (rhs_scope, rhs_match) = (y s lhs_scope) in
+    (rhs_scope, (lhs_match; rhs_match))))"
+
+abbreviation decend where
+  "decend f e v \<equiv> (\<lambda>s s'. f e (snd (fresh v s)) s')"
+
+value "match \<langle> fresh STR ''e''"
+
+fun register_name where
+  "register_name (s, m) vn v = (s, m(vn:=Some v))"
+
+fun match_pattern :: "IRExpr \<Rightarrow> VarName \<Rightarrow> Scope \<Rightarrow> Scope \<times> MATCH" where
+  "match_pattern (UnaryExpr op e) v =
+    match v \<langle>
+      (UnaryPattern op \<langle> fresh STR ''a'')
+    |> decend match_pattern e STR ''a''
+    " |
+  "match_pattern (BinaryExpr op e1 e2) v =
+    (match v \<langle> 
+      (BinaryPattern op \<langle> fresh STR ''a'' \<rangle> fresh STR ''b'')
+    |> decend match_pattern e1 STR ''a'')
+    |> decend match_pattern e2 STR ''b''" |
+  "match_pattern (ConditionalExpr b e1 e2) v =
+    ((match v \<langle>
+      ((ConditionalPattern \<langle> fresh STR ''a'' \<rangle> fresh STR ''b'') \<rangle> fresh STR ''c'')
+    |> decend match_pattern b STR ''a'')
+    |> decend match_pattern e1 STR ''b'')
+    |> decend match_pattern e2 STR ''c''" |
+  "match_pattern (VariableExpr vn st) v = 
+    (\<lambda>s. (case (snd s) vn of 
+      None \<Rightarrow> (register_name s vn v, noop) |
+      Some v' \<Rightarrow> (register_name s vn v, v' == v)))"
+
+fun expr_result :: "IRExpr \<Rightarrow> Scope \<Rightarrow> IRExpr" where
+  "expr_result (UnaryExpr op e) s = 
+    UnaryExpr op (expr_result e s)" |
+  "expr_result (BinaryExpr op e1 e2) s = 
+    BinaryExpr op (expr_result e1 s) (expr_result e2 s)" |
+  "expr_result (ConditionalExpr b e1 e2) s = 
+    ConditionalExpr (expr_result b s) (expr_result e1 s) (expr_result e2 s)" |
+  "expr_result (VariableExpr vn st) (s, m) = 
+    (case m vn of None \<Rightarrow> VariableExpr vn st 
+                | Some v' \<Rightarrow> VariableExpr v' st)" |
+  "expr_result e v = e"
+
+fun generate :: "IRExpr \<Rightarrow> IRExpr \<Rightarrow> MATCH \<times> IRExpr" where
+  "generate p r = 
+    (let (s, m) = match_pattern p STR ''e'' ({||}, (\<lambda>x. None))
+     in (m, expr_result r s))"
+
+value
+  "generate 
+    (UnaryExpr UnaryNot
+      (UnaryExpr UnaryNot (var ''x'')))
+    (var ''x'')"
+
+value
+  "generate 
+    (BinaryExpr BinAdd
+      (BinaryExpr BinSub (var ''x'') (var ''y''))
+      (var ''y''))
+    (var ''x'')"
+
+code_printing
+  type_constructor MATCH \<rightharpoonup> (Scala) "MATCH"
+  | constant match \<rightharpoonup> (Scala) "match"
+  | constant seq \<rightharpoonup> (Scala) "seq"
+  | constant noop \<rightharpoonup> (Scala) "noop"
+  | constant equality \<rightharpoonup> (Scala) "=="
+
+definition redundant_sub where
+  "redundant_sub = generate 
+    (BinaryExpr BinAdd
+      (BinaryExpr BinSub (var ''x'') (var ''y''))
+      (var ''y''))
+    (var ''x'')"
+
+definition redundant_sub_gen where
+  "redundant_sub_gen = ((((MATCH.match STR ''e''
+   (BinaryPattern BinAdd STR ''a''
+     STR ''b''); MATCH.match STR ''a''
+                  (BinaryPattern BinSub STR ''az'' STR ''bz'')); noop); noop); STR ''bz'' == STR ''b'',
+  VariableExpr STR ''az'' VoidStamp)"
+
+export_code redundant_sub in Scala
+export_code redundant_sub_gen in Scala
+
+(*
+fun generate :: "Vars \<Rightarrow> IRExpr \<times> IRExpr \<times> (Substitution \<Rightarrow> bool) \<Rightarrow> MATCH" where
+  "generate s (UnaryExpr op e, e', f) =
+    (let
+      used = s |\<union>| {|(fresh (STR ''e'') s), (fresh (STR ''ea'') s)|}
+     in
+        ((match (fresh (STR ''e'') s) (UnaryPattern op (fresh (STR ''ea'') s)));
+        (generate used (e, e', f))))" |
+  "generate s (BinaryExpr op e1 e2, e', f) = 
+    (let 
+      used = (s |\<union>| {|(fresh STR ''e'' s), (fresh STR ''ea'' s), (fresh STR ''eb'' s)|})
+     in
+        (((match (fresh STR ''e'' s)
+            (BinaryPattern op (fresh (STR ''ea'') s) (fresh (STR ''eb'') s)));
+        (generate used (e1, e', f)));
+        (generate used (e2, e', f))))" |
+  "generate s (ConditionalExpr b e1 e2, e', f) = 
+    (let
+      used = (s |\<union>| {|(fresh STR ''e'' s), (fresh STR ''ea'' s), (fresh STR ''eb'' s), (fresh STR ''ec'' s)|})
+     in
+        (((match (fresh STR ''e'' s)
+              (ConditionalPattern (fresh (STR ''ea'') s) (fresh (STR ''eb'') s) (fresh (STR ''ec'') s)));
+          ((generate used (b, e', f));
+          ((generate used (e1, e', f));
+           (generate used (e2, e', f)))))))" |
+  "generate s (e, e', f) = match (fresh STR ''e'' s) (VariablePattern STR ''e'')"
+
+value "generate {||} (BinaryExpr BinAdd (var ''x'') (var ''y''), var ''x'', \<lambda>x. True)"
+
+value
+  "generate {||} 
+    (BinaryExpr BinAdd
+      (BinaryExpr BinSub x y)
+       y,
+     x, \<lambda>x. True)"
+
+value
+  "generate {||} 
+    (BinaryExpr BinAdd
+      (BinaryExpr BinSub (var ''x'') (var ''y''))
+      (var ''y''),
+     (var ''x''), \<lambda>x. True)"
+
+fun replace :: "MatchRules \<Rightarrow> IRExpr \<Rightarrow> IRExpr option" where
+  "replace (match_pattern p) e = (if (match (Rep_PatternExpr p) e \<noteq> None) then Some e else None) " |
+  "replace (ground g) e = Some g" |
+  "replace (conditional c t f) e = (if (replace c e) \<noteq> None then (replace t e) else (replace f e))" |
+  "replace (fail) e = None"
+
+(*
+  "generate (ConditionalExpr b e1 e2) = 1 + max (pattern_depth b) (max (pattern_depth e1) (pattern_depth e2))" |
+  "generate (ParameterExpr i s) = 1" |
+  "generate (LeafExpr n s) = 1" |
+  "generate (ConstantExpr v) = 1" |
+  "generate (ConstantVar x) = 0" |
+  "generate (VariableExpr x s) = 0"*)
+code_datatype Abs_PatternExpr
+code_datatype Abs_GroundExpr
+
+value "generate {} ( (VariableExpr (STR ''x'') VoidStamp), (ConstantExpr (IntVal 32 0)), \<lambda>_.True)"
+(*
+value "replace (generate ( (VariableExpr (STR ''x'') VoidStamp), (ConstantExpr (IntVal32 0)), \<lambda>_.True)) (ConstantExpr (IntVal32 0))"
+*)
+
+value "generate ((ConstantExpr (IntVal 32 0)), (ConstantExpr (IntVal 32 0)), \<lambda>_.True)"
+value "generate ((UnaryExpr UnaryAbs (ConstantExpr (IntVal 32 0))), (ConstantExpr (IntVal 32 0)), \<lambda>_.True)"
+value "generate ((UnaryExpr UnaryAbs (VariableExpr (STR ''x'') VoidStamp)), (ConstantExpr (IntVal 32 0)), \<lambda>_.True)"
+
+
+(*
+definition f where "f = generate ((BinaryExpr BinAnd
+    (BinaryExpr BinOr (VariableExpr STR ''x'' (IntegerStamp 1 (fst (bit_bounds 1)) (snd (bit_bounds 1))))
+      (VariableExpr STR ''y'' (IntegerStamp 1 (fst (bit_bounds 1)) (snd (bit_bounds 1)))))
+    (VariableExpr STR ''z'' (IntegerStamp 1 (fst (bit_bounds 1)) (snd (bit_bounds 1))))),
+   (BinaryExpr BinAnd (VariableExpr STR ''x'' (IntegerStamp 1 (fst (bit_bounds 1)) (snd (bit_bounds 1))))
+    (VariableExpr STR ''z'' (IntegerStamp 1 (fst (bit_bounds 1)) (snd (bit_bounds 1))))), (\<lambda>_.True))"
+
+export_code f in SML
+value "f"*)
+
+definition example_rewrite :: Rewrite where
+  "example_rewrite = TermRewrites.Rewrite.Abs_Rewrite
+  (BinaryExpr BinAnd
+    (BinaryExpr BinOr (VariableExpr STR ''x'' (IntegerStamp 1 (fst (bit_bounds 1)) (snd (bit_bounds 1))))
+      (VariableExpr STR ''y'' (IntegerStamp 1 (fst (bit_bounds 1)) (snd (bit_bounds 1)))))
+    (VariableExpr STR ''z'' (IntegerStamp 1 (fst (bit_bounds 1)) (snd (bit_bounds 1)))),
+   BinaryExpr BinAnd (VariableExpr STR ''x'' (IntegerStamp 1 (fst (bit_bounds 1)) (snd (bit_bounds 1))))
+    (VariableExpr STR ''z'' (IntegerStamp 1 (fst (bit_bounds 1)) (snd (bit_bounds 1)))),
+   \<lambda>x. True)"
+
+lift_definition generate_rewrite :: "Rewrite \<Rightarrow> MatchRules"
+  is generate .
+
+
+
+
+value "generate_rewrite example_rewrite"
+
+experiment begin
 lemma match_succeeds:
   assumes "match e1 e = Some \<sigma>"
   shows "\<sigma> $ e1 = e"
-  and "vars e1 = dom \<sigma>"
-(*proof (induct e arbitrary: \<sigma> e1 rule: match.induct) *)
-sorry
+  and "fset (vars e1) = dom \<sigma>"
+  using assms
+   apply (induct e1 e arbitrary: \<sigma> rule: match.induct; auto)
+                 apply (meson option.distinct(1))+
+  sorry
+
 
 definition isIntExpr :: "IRExpr \<Rightarrow> bool" where
-  "isIntExpr e = (\<forall>m p v. ([m, p] \<turnstile> e \<mapsto> v) \<longrightarrow> is_IntVal32 v)"
+  "isIntExpr e = (\<forall>m p v. ([m, p] \<turnstile> e \<mapsto> v) \<longrightarrow> is_IntVal v)"
 
 lemma int_add_preserve:
-  assumes "is_IntExpr ex"
-  assumes "is_IntExpr ey"
-  shows "isIntExpr (BinaryAdd BinAdd ex ey)"
+  assumes "isIntExpr ex"
+  assumes "isIntExpr ey"
+  shows "isIntExpr (BinaryExpr BinAdd ex ey)"
   sorry
 
-lemma "valid_value (constantAsStamp (IntVal32 v)) (IntVal32 v)"
+lemma valid_constant: "valid_value (IntVal 32 v) (constantAsStamp (IntVal 32 v))"
   sorry
 
-lemma int_constant: "isIntExpr (ConstantExpr (IntVal32 v))"
+lemma int_constant: "isIntExpr (ConstantExpr (IntVal 32 v))"
   sorry
 
-lemma "isIntExpr e \<Longrightarrow> (\<exists>v. \<forall>m p. [m, p] \<turnstile> e \<mapsto> IntVal32 v)"
+lemma "isIntExpr e \<Longrightarrow> (\<exists>v. \<forall>m p. [m, p] \<turnstile> e \<mapsto> IntVal 32 v)"
   sorry
 
 lemma var_x: 
-  assumes "\<forall>e \<sigma>. match (BinaryExpr BinAdd (VariableExpr ''x'' IntStamp32) (ConstantExpr (IntVal32 0))) e = Some \<sigma>"
-  shows "''x'' \<in> vars (BinaryExpr BinAdd (VariableExpr ''x'' IntStamp32) (ConstantExpr (IntVal32 0)))"
+  assumes "\<forall>e \<sigma>. match (BinaryExpr BinAdd (VariableExpr STR ''x'' IntStamp32) (ConstantExpr (IntVal 32 0))) e = Some \<sigma>"
+  shows "STR ''x'' |\<in>| vars (BinaryExpr BinAdd (VariableExpr STR ''x'' IntStamp32) (ConstantExpr (IntVal 32 0)))"
     using vars.simps by simp
 
 lemma domx: 
-  assumes "match (BinaryExpr BinAdd (VariableExpr ''x'' IntStamp32) (ConstantExpr (IntVal32 0))) e = Some \<sigma>" 
-  shows "''x'' \<in> dom \<sigma>"
-    using match_succeeds(2) var_x
-    by (metis assms insertI1 insert_is_Un vars.simps(2) vars.simps(8))
+  assumes "match (BinaryExpr BinAdd (VariableExpr STR ''x'' IntStamp32) (ConstantExpr (IntVal 32 0))) e = Some \<sigma>" 
+  shows "STR ''x'' \<in> dom \<sigma>"
+    using match_succeeds(2) var_x sorry(*
+    by (metis assms insertI1 insert_is_Un vars.simps(2) vars.simps(8))*)
 
 lemma zero_helper_x:
-  assumes "match (BinaryExpr BinAdd (VariableExpr ''x'' IntStamp32) (ConstantExpr (IntVal32 0))) e = Some \<sigma>"
-  shows "\<sigma> ''x'' \<noteq> SubNone"
+  assumes "match (BinaryExpr BinAdd (VariableExpr STR ''x'' IntStamp32) (ConstantExpr (IntVal 32 0))) e = Some \<sigma>"
+  shows "maps_to \<sigma> STR ''x'' \<noteq> None"
   using domx in_dom assms by presburger
 
 lemma zero_identity: 
-  "rewrite_valid_rep (BinaryExpr BinAdd (VariableExpr ''x'' IntStamp32) (ConstantExpr (IntVal32 0))) 
-                     (VariableExpr ''x'' IntStamp32)"
+  "rewrite_valid_rep (BinaryExpr BinAdd (VariableExpr STR ''x'' IntStamp32) (ConstantExpr (IntVal 32 0))) 
+                     (VariableExpr STR ''x'' IntStamp32)"
 proof -
-  have pv: "\<forall>vx. intval_add (IntVal32 vx) (IntVal32 0) = IntVal32 vx" 
-    using intval_add.simps by simp
-  have vvx: "valid_value (constantAsStamp (IntVal32 0)) (IntVal32 0)"
+  have pv: "\<forall>vx. intval_add (IntVal 32 vx) (IntVal 32 0) = IntVal 32 vx" 
+    using intval_add.simps
+    using valid_constant by auto
+  have vvx: "valid_value (IntVal 32 0) (constantAsStamp (IntVal 32 0))"
     using valid_constant by blast
-  have eval0: "\<forall>m p. [m, p] \<turnstile> ConstantExpr (IntVal32 0) \<mapsto> (IntVal32 0)"
-    using ConstantExpr vvx by blast
+  have eval0: "\<forall>m p. [m, p] \<turnstile> ConstantExpr (IntVal 32 0) \<mapsto> (IntVal 32 0)"
+    using ConstantExpr vvx
+    using wf_value_def by blast
   have eval_add: "\<forall>ex. isIntExpr ex \<longrightarrow> 
-    (\<forall>m p vx. ([m, p] \<turnstile> ex \<mapsto> IntVal32 vx) \<longrightarrow> 
-      ([m, p] \<turnstile> BinaryExpr BinAdd ex (ConstantExpr (IntVal32 0)) \<mapsto> (IntVal32 vx)))"
+    (\<forall>m p vx. ([m, p] \<turnstile> ex \<mapsto> IntVal 32 vx) \<longrightarrow> 
+      ([m, p] \<turnstile> BinaryExpr BinAdd ex (ConstantExpr (IntVal 32 0)) \<mapsto> (IntVal 32 vx)))"
     by (metis BinaryExpr Value.distinct(1) bin_eval.simps(1) eval0 pv)
   have add_eval: "\<forall>ex. isIntExpr ex \<longrightarrow>
-      (\<forall>m p v. ([m, p] \<turnstile> BinaryExpr BinAdd ex (ConstantExpr (IntVal32 0)) \<mapsto> v) \<longrightarrow> 
+      (\<forall>m p v. ([m, p] \<turnstile> BinaryExpr BinAdd ex (ConstantExpr (IntVal 32 0)) \<mapsto> v) \<longrightarrow> 
                [m, p] \<turnstile> ex \<mapsto> v)"
-    using eval_add evalDet by (metis BinaryExprE isIntExpr_def is_IntVal32_def) 
+    using eval_add evalDet sorry
   have add_refine: "\<forall>ex. isIntExpr ex \<longrightarrow>
-      BinaryExpr BinAdd ex (ConstantExpr (IntVal32 0)) \<ge> ex"
+      BinaryExpr BinAdd ex (ConstantExpr (IntVal 32 0)) \<ge> ex"
     unfolding le_expr_def
     using add_eval by blast
-  have add_refine_substit: "\<forall>\<sigma> ex. \<sigma> ''x'' = SubExpr ex \<and> isIntExpr ex \<longrightarrow>
-        BinaryExpr BinAdd ex (ConstantExpr (IntVal32 0)) \<ge> ex"
+  have add_refine_substit: "\<forall>\<sigma> ex. \<sigma> STR ''x'' = SubExpr ex \<and> isIntExpr ex \<longrightarrow>
+        BinaryExpr BinAdd ex (ConstantExpr (IntVal 32 0)) \<ge> ex"
     using add_refine by blast
-  have add_substit: "\<forall>\<sigma> ex. \<sigma> ''x'' = SubExpr ex \<and> isIntExpr ex \<longrightarrow>
-        \<sigma> $ (BinaryExpr BinAdd (VariableExpr ''x'' IntStamp32) (ConstantExpr (IntVal32 0))) \<ge> ex"
+  have add_substit: "\<forall>\<sigma> ex. maps_to \<sigma> STR ''x'' = Some (SubExpr ex) \<and> isIntExpr ex \<longrightarrow>
+        \<sigma> $ (BinaryExpr BinAdd (VariableExpr STR ''x'' IntStamp32) (ConstantExpr (IntVal 32 0))) \<ge> ex"
     using add_refine_substit by fastforce
-  have match_e: "\<forall>e \<sigma>. match (BinaryExpr BinAdd (VariableExpr ''x'' IntStamp32) (ConstantExpr (IntVal32 0))) e = (Some \<sigma>) \<longrightarrow>
-         (e = \<sigma> $ (BinaryExpr BinAdd (VariableExpr ''x'' IntStamp32) (ConstantExpr (IntVal32 0))))"
+  have match_e: "\<forall>e \<sigma>. match (BinaryExpr BinAdd (VariableExpr STR ''x'' IntStamp32) (ConstantExpr (IntVal 32 0))) e = (Some \<sigma>) \<longrightarrow>
+         (e = \<sigma> $ (BinaryExpr BinAdd (VariableExpr STR ''x'' IntStamp32) (ConstantExpr (IntVal 32 0))))"
     using match_succeeds match.simps(7) by presburger
-  have v: " vars (BinaryExpr BinAdd (VariableExpr ''x'' IntStamp32) (ConstantExpr (IntVal32 0))) \<subseteq> vars (VariableExpr ''x'' IntStamp32)"
+  have v: " vars (BinaryExpr BinAdd (VariableExpr STR ''x'' IntStamp32) (ConstantExpr (IntVal 32 0))) |\<subseteq>| vars (VariableExpr STR ''x'' IntStamp32)"
     using vars.simps  by simp
-  have "\<forall>\<sigma> e. vars (BinaryExpr BinAdd (VariableExpr ''x'' IntStamp32) (ConstantExpr (IntVal32 0))) \<subseteq> vars (VariableExpr ''x'' IntStamp32) \<longrightarrow>
-        match (BinaryExpr BinAdd (VariableExpr ''x'' IntStamp32) (ConstantExpr (IntVal32 0))) e = Some \<sigma> \<longrightarrow>
-        \<sigma> $ VariableExpr ''x'' IntStamp32 \<le> e"
+  have "\<forall>\<sigma> e. vars (BinaryExpr BinAdd (VariableExpr STR ''x'' IntStamp32) (ConstantExpr (IntVal 32 0))) |\<subseteq>| vars (VariableExpr STR ''x'' IntStamp32) \<longrightarrow>
+        match (BinaryExpr BinAdd (VariableExpr STR ''x'' IntStamp32) (ConstantExpr (IntVal 32 0))) e = Some \<sigma> \<longrightarrow>
+        \<sigma> $ VariableExpr STR ''x'' IntStamp32 \<le> e"
     apply simp
     using match_e add_substit  sorry
-  have dom: "\<forall>e \<sigma>. match (BinaryExpr BinAdd (VariableExpr ''x'' IntStamp32) (ConstantExpr (IntVal32 0))) e = Some \<sigma> \<longrightarrow> 
-            vars (BinaryExpr BinAdd (VariableExpr ''x'' IntStamp32) (ConstantExpr (IntVal32 0))) \<subseteq> dom \<sigma>"
+  have dom: "\<forall>e \<sigma>. match (BinaryExpr BinAdd (VariableExpr STR ''x'' IntStamp32) (ConstantExpr (IntVal 32 0))) e = Some \<sigma> \<longrightarrow> 
+            fset (vars (BinaryExpr BinAdd (VariableExpr STR ''x'' IntStamp32) (ConstantExpr (IntVal 32 0)))) \<subseteq> dom \<sigma>"
     using match_succeeds by (metis dual_order.refl)
 
   show ?thesis 
     unfolding rewrite_valid_rep_def
     sorry
 qed
+end
+*)
 
 end
